trying with list of expressions, induction too weak

src/Typing.v
@@ -20,6 +20,12 @@ Require Import List.
 Require Import SimpleTypes.
 Require Import MyLtacs.
 
+(** * Pattern definition *)
+
+Inductive pat : Set :=
+| var_p : id -> pat
+| const_p : id -> pat.
+
 (** * Lambda term definition *)
 
 Inductive term : Set :=
@@ -27,9 +33,36 @@ Inductive term : Set :=
 | app_t   : term -> term -> term
 | let_t   : id -> term -> term -> term
 | lam_t   : id -> term -> term
-| const_t : id -> term.
+| const_t : id -> term
+| case_t  : term -> pat -> term -> list pat -> list term -> term.
+
+Inductive has_type_pat : ctx -> pat -> ty -> Prop:=
+| const_htp : forall x G, has_type_pat G (const_p x) (con x)
+| var_htp : forall x G sigma tau, in_ctx x G = Some sigma -> is_schm_instance tau sigma ->
+                            has_type_pat G (var_p x) tau.
+
+Inductive has_type_patterns : ctx -> list pat -> ty -> Prop :=
+| one_pattern : forall G p tau, has_type_pat G p tau ->
+                           has_type_patterns G (p::nil) tau
+| many_pattern : forall G p ps tau, has_type_pat G p tau ->
+                               has_type_patterns G ps tau ->
+                               has_type_patterns G (p::ps) tau.
 
 (** * Syntax-directed rule system of Damas-Milner *)
+
+Fixpoint get_pats (c : list (pat * term)) : list pat :=
+  match c with
+  | nil => nil
+  | (p, _)::c' => p::get_pats c'
+  end.
+
+Fixpoint get_terms (c : list (pat * term)) : list term :=
+  match c with
+  | nil => nil
+  | (_, t)::c' => t::get_terms c'
+  end.
+
+
 
 Inductive has_type : ctx -> term -> ty -> Prop :=
 | const_ht : forall x G, has_type G (const_t x) (con x)
@@ -42,14 +75,29 @@ Inductive has_type : ctx -> term -> ty -> Prop :=
                                has_type G (app_t l rho) tau'
 | let_ht : forall G x e e' tau tau', has_type G e tau ->
                                 has_type ((x, gen_ty tau G) :: G) e' tau' ->
-                                has_type G (let_t x e e') tau'.
+                                has_type G (let_t x e e') tau'
+| case_ht : forall G e p t tau tau' ps ts, has_type G e tau ->
+                                    has_type_pat G p tau ->
+                                    has_type G t tau' ->
+                                    Forall (fun p' => has_type_pat G p' tau) ps ->
+                                    Forall (fun t' => has_type G t' tau) ts ->
+                                    has_type G (case_t e p t (com) tau'.
+                                         (*
+| case_many_ht : forall G e p t cs tau tau', has_type G e tau ->
+                                        has_type_pat G p tau ->
+                                        has_type G t tau' ->
+                                        has_type G (case_t e cs) tau' ->
+                                        has_type G (case_t e ((p, t)::cs)) tau'.
+*)
 
 (** * The Great Substitution Lemma *)
-(** has_type is stable under substitution *)
-Lemma has_type_is_stable_under_substitution : forall e s G tau,
-    has_type G e tau -> has_type (apply_subst_ctx s G) e (apply_subst s tau).
+
+(** has_pat is stable under substitution *)
+Lemma has_type_pat_is_stable_under_substitution : forall e s G tau,
+    has_type_pat G e tau -> has_type_pat (apply_subst_ctx s G) e (apply_subst s tau).
 Proof.
   induction e.
+  (** var case *)
   - intros. inversion H.
     subst.
     econstructor.
@@ -66,6 +114,69 @@ Proof.
       eapply subst_inst_subst_type in H0.
       exists (map_apply_subst_ty s x).
       apply H0.
+  (** const case *)
+  - intros. inversion H.
+    subst.
+    econstructor.
+Qed.
+
+Hint Resolve has_type_pat_is_stable_under_substitution.
+
+(** has_patterns is stable under substitution *)
+Lemma has_type_patterns_is_stable_under_substitution : forall l s G tau,
+    has_type_patterns G l tau -> has_type_patterns (apply_subst_ctx s G) l (apply_subst s tau).
+Proof.
+  induction l.
+  - intros. inverts H.
+  - intros. 
+    inverts* H.
+    econstructor.
+    auto.
+    econstructor.
+    auto.
+    auto.
+Qed.    
+
+Hint Resolve has_type_patterns_is_stable_under_substitution.
+
+(*
+Lemma has_type_list_stabe : forall G tau l s,
+    Forall (fun t' => has_type G t' tau) l ->
+    Forall (fun t' => has_type (apply_subst_ctx s G) t' (apply_subst s tau)) l. 
+Proof.
+  induction l.
+  - intros.
+    auto.
+  - intros.
+    inverts* H.
+    econstructor.
+*)
+    
+
+
+(** has_type is stable under substitution *)
+Lemma has_type_is_stable_under_substitution : forall e s G tau,
+    has_type G e tau -> has_type (apply_subst_ctx s G) e (apply_subst s tau).
+Proof.
+  induction e.
+  (** var case *)
+  - intros. inversion H.
+    subst.
+    econstructor.
+    + induction G; simpl in *; mysimp.
+      destruct a.
+      mysimp.
+      apply IHG.
+      econstructor.
+      apply H1.
+      assumption.
+      assumption.
+    + unfold is_schm_instance in *.
+      destruct H3.
+      eapply subst_inst_subst_type in H0.
+      exists (map_apply_subst_ty s x).
+      apply H0.
+  (** app case *)
   - intros. 
     inversion H.
     subst.
@@ -75,6 +186,7 @@ Proof.
     assumption.
     apply IHe2.
     assumption.
+  (** let case *)
   - intros. 
     inversion H.
     subst.
@@ -103,12 +215,118 @@ Proof.
     erewrite <- gen_ty_renaming.
     assumption.
     apply r.
+  (** lam case *)
   - intros. inversion H. subst. rewrite apply_subst_arrow.
     econstructor. rewrite <- ty_to_subst_schm. rewrite apply_subst_ctx_eq. apply IHe.
     assumption.
+  (** const case *)
   - intros. inversion H.
     subst.
     econstructor.
+  (** case case *)
+  - intros.
+    induction l.
+    + intros. inverts* H.
+      econstructor; eauto.
+      apply Forall_forall.
+      intros.
+      inverts* H.
+      apply Forall_forall.
+      intros.
+      inverts* H.
+    + inverts* H.
+      apply case_ht with (tau:= apply_subst s tau0). 
+      * eapply IHe1 with (s:=s) in H4.
+        auto.
+      * auto.
+      * auto.
+      * apply Forall_forall.
+        intros.
+        destruct a.
+        simpl in *.
+        destruct H.
+        {
+          subst. 
+          eapply Forall_forall with (x:=x) in H9.
+          auto.
+          simpl. left. auto.
+        }
+        {
+          eapply Forall_forall with (x:=x) in H9.
+          auto.
+          simpl. right. auto.
+        }
+      * apply Forall_forall.
+        destruct a.
+        simpl in *.
+        intros.
+        destruct H.
+        {
+          subst. 
+          eapply Forall_forall with (x:=x) in H10.
+          auto.
+          simpl. left. auto.
+        }
+        {
+          eapply Forall_forall with (x:=x) in H9.
+          auto.
+          simpl. right. auto.
+        }
+        intros.
+
+      *
+
+      {
+        induction t.
+        - skip.
+        - skip.
+        - skip.
+        - skip.
+        - skip.
+        - destruct l.
+          + inverts* H7.
+          + inverts* H7.
+            econstructor.
+            apply 
+          + destruct p0.
+            econstructor.
+            apply IHt; auto.
+          
+            
+      (*aqui*)
+        
+      apply IHl in H8.
+      econstructor.
+      apply IHe.
+      apply H3.
+      auto.
+      skip.
+      auto.
+    + econstructor; eauto.
+      skip.
+
+      
+    + destruct a as [p t].
+      * econstructor; eauto.
+      eapply IHe.
+      apply H2.
+      auto.
+      apply Forall_forall.
+      intros.
+      simpl in *.
+      destruct H.
+      * subst.
+        inverts* H6.
+        skip.
+      * inverts* H6.
+      
+       
+      inverts* H6.
+      inverts* H4.
+      auto.
+      apply IHe.
+      apply has_type_patterns_is_stable_under_substitution.
+      inverts* H6.
 Qed.
 
 Hint Resolve has_type_is_stable_under_substitution.
